theories/examples/pool_quicksort.v
@@ -8,6 +8,8 @@ From zoo.diaframe Require Import
   diaframe.
 From zoo_std Require Export
   array.
+From zoo_std Require Import
+  for_.
 From zoo_parabs Require Import
   pool.
 From examples Require Export
@@ -18,64 +20,207 @@ From zoo Require Import
 Section pool_G.
   Context `{pool_G : PoolG}.
 
-  #[local] Lemma pool_quicksort_partition_spec arr i i_ ns sz :
+  #[local] Lemma pool_quicksort_partition_spec arr i i_ xs sz :
     (0 ≤ i)%Z →
     i_ = ₊i →
     (1 < sz)%Z →
-    length ns = ₊sz →
+    length xs = ₊sz →
     {{{
-      array_slice arr i_ (DfracOwn 1) (#*@{Z} ns)
+      array_slice arr i_ (DfracOwn 1) (#*@{Z} xs)
     }}}
       pool_quicksort_partition arr #i #sz
     {{{
-      ns1 p pivot ns2
+      xs1 p pivot xs2
     , RET #p;
-      ⌜p = (i_ + length ns1)%nat⌝ ∗
-      ⌜ns ≡ₚ ns1 ++ pivot :: ns2⌝ ∗
-      ⌜Forall ((≥)%Z pivot) ns1⌝ ∗
-      ⌜Forall ((≤)%Z pivot) ns2⌝ ∗
-      array_slice arr i_ (DfracOwn 1) (#*@{Z} ns1 ++ #@{Z} pivot :: #*@{Z} ns2)
+      ⌜p = (i_ + length xs1)%nat⌝ ∗
+      ⌜xs ≡ₚ xs1 ++ pivot :: xs2⌝ ∗
+      ⌜Forall ((≥)%Z pivot) xs1⌝ ∗
+      ⌜Forall ((≤)%Z pivot) xs2⌝ ∗
+      array_slice arr i_ (DfracOwn 1) (#*@{Z} xs1 ++ #@{Z} pivot :: #*@{Z} xs2)
     }}}.
   Proof.
-  Admitted.
+    iIntros (Hi -> Hsz Hxs) "%Φ Harr HΦ".
 
-  #[local] Lemma pool_quicksort_main_0_spec pool ctx scope arr i i_ ns sz :
+    destruct xs as [| pivot xs]; simpl in Hxs. 1: lia.
+    iEval (rewrite fmap_cons) in "Harr".
+    iDestruct (array_slice_cons_1 with "Harr") as "(Harr_1 & Harr_2)".
+
+    wp_rec.
+    wp_apply+ (array_unsafe_get_spec_cell with "Harr_1") as "Harr_1". 1: lia.
+    wp_ref r as "Hr".
+
+    wp_apply+ (for_spec_strong (λ j _,
+      ∃ xs' (i1 : Z),
+      array_slice arr (S ₊i) (DfracOwn 1) (#*@{Z} xs') ∗
+      r ↦ᵣ #i1 ∗
+      ⌜xs ≡ₚ xs'⌝ ∗
+      ⌜i < i1 ≤ j⌝%Z ∗
+      ⌜ ∀ (k : nat) x,
+        xs' !! k = Some x →
+        (k < i1 - i - 1)%Z →
+        (x ≤ pivot)%Z
+      ⌝ ∗
+      ⌜ ∀ (k : nat) x,
+        xs' !! k = Some x →
+        (i1 - i - 1 ≤ k < j - i - 1)%Z →
+        (pivot ≤ x)%Z
+      ⌝
+    )%I with "[Harr_2 Hr]") as "(%xs' & %i1 & Harr_2 & Hr & %Hxs' & %Hi1 & %H1 & %H2)".
+    { iSplitL.
+      { iFrame. iPureIntro. auto with lia. }
+
+      iIntros "!> %i2 %𝑖2 % % (%xs' & %i1 & Harr & Hr & %Hxs' & %Hi1 & %H1 & %H2)".
+      destruct (lookup_lt_is_Some_2 xs' ₊(i1 - i - 1)) as (x1 & Hlookup_1).
+      { rewrite -Hxs'. lia. }
+      destruct (lookup_lt_is_Some_2 xs' 𝑖2) as (x2 & Hlookup_2).
+      { rewrite -Hxs'. lia. }
+
+      wp_apply+ (array_unsafe_get_spec_slice with "Harr") as "Harr".
+      { lia. }
+      { apply list_lookup_fmap_Some_2 => //. }
+      { lia. }
+
+      wp_pures.
+      case_bool_decide as Hx2; wp_pures.
+
+      - wp_load.
+
+        wp_apply (array_unsafe_swap_spec_slice ₊(i1 - i - 1) with "Harr") as "Harr".
+        1,2,4: lia.
+        1,2: apply list_lookup_fmap_Some_2 => //.
+        1: lia.
+        iEval (rewrite -!list_fmap_insert) in "Harr".
+
+        iStep 15. iPureIntro. split_and!.
+        { rewrite Permutation_swap' //. }
+        { lia. }
+        { lia. }
+        all:
+          intros k x
+            [ (<- & <- & _)
+            | ( ?
+              & [ (<- & <- & _)
+                | (? & Hlookup_k)
+                ]%list_lookup_insert_Some
+              )
+            ]%list_lookup_insert_Some Hk.
+        { destruct_decide (𝑖2 = ₊(i1 - i - 1)) as -> | ?.
+          - congruence.
+          - lia.
+        }
+        all: naive_solver lia.
+
+      - iStep 6. iPureIntro.
+        intros k x Hlookup_k Hk.
+        destruct_decide (k = 𝑖2) as -> | Hcase.
+        all: naive_solver lia.
+    }
+
+    rewrite Z.max_r in Hi1 H2. 1: lia.
+    apply Permutation_length in Hxs' as ?.
+
+    iDestruct (array_slice_cons_2 with "Harr_1 Harr_2") as "Harr".
+
+    wp_load. wp_pures.
+
+    destruct_decide (i1 = i + 1)%Z as -> | Hcase.
+
+    - wp_apply+ (array_unsafe_swap_spec_slice_id with "Harr") as "Harr". 1,2: simpl; lia.
+      iSteps as "_".
+
+      iEval (replace _ with ⁺₊i by lia).
+      iApply ("HΦ" $! [] ₊i pivot xs').
+      iSteps; iPureIntro.
+      { rewrite Hxs' //. }
+      { apply Forall_lookup. intros k x Hlookup.
+        apply lookup_lt_Some in Hlookup as ?.
+        eapply H2; [done | lia].
+      }
+
+    - assert (
+        ∃ xs1 xs2,
+        xs' = xs1 ++ xs2 ∧
+        length xs1 = ₊(i1 - i - 1) ∧
+        Forall ((≥)%Z pivot) xs1 ∧
+        length xs2 = ₊(i + length xs + 1 - i1) ∧
+        Forall ((≤)%Z pivot) xs2
+      ) as (xs1 & xs2 & -> & Hxs1_length & Hxs1 & Hxs2_length & Hxs2).
+      { exists (take ₊(i1 - i - 1) xs'), (drop ₊(i1 - i - 1) xs'). split_and!.
+        - rewrite take_drop //.
+        - simpl_length. lia.
+        - apply Forall_lookup. intros k x (Hlookup & Hk)%lookup_take_Some.
+          eapply Z.le_ge, H1; [done | lia].
+        - simpl_length. lia.
+        - apply Forall_lookup. intros k x Hlookup.
+          rewrite lookup_drop in Hlookup.
+          apply lookup_lt_Some in Hlookup as ?.
+          eapply H2; [done | lia].
+      }
+      iEval (rewrite fmap_app) in "Harr".
+
+      destruct xs1 as [| x xs1 _] using rev_ind. 1: naive_solver lia.
+      simpl_length/= in Hxs1_length.
+      iEval (rewrite fmap_app /=) in "Harr".
+
+      iDestruct (array_slice_app_2 (_ :: _) with "Harr") as "(Harr_1 & Harr_2)". 1: done.
+      wp_apply+ (array_unsafe_swap_spec_slice 0 ₊(i1 - i - 1) with "Harr_1") as "Harr_1". 1-4,6: auto with lia.
+      { apply lookup_cons_r_Some. 1: lia.
+        apply lookup_app_r_Some; simpl_length. 1: lia.
+        replace _ with 0 by lia. done.
+      }
+      iEval (rewrite /= insert_cons_r; first lia) in "Harr_1".
+      iEval (rewrite insert_app_r_alt; first (simpl_length; lia)) in "Harr_1".
+      iEval (simpl_length) in "Harr_1".
+      iEval (rewrite insert_cons_l; first lia) in "Harr_1".
+      iDestruct (array_slice_app_1' with "Harr_1 Harr_2") as "Harr". 1: simpl_length/=.
+      iEval (rewrite -(assoc _ (_ :: _))) in "Harr".
+
+      wp_load. wp_pures.
+
+      iEval (rewrite -(Z2Nat.id (i1 - 1)); first lia).
+      iApply ("HΦ" $! (x :: xs1) _ pivot xs2).
+      iFrameSteps; iPureIntro.
+      { rewrite Hxs'. solve_Permutation. }
+      { rewrite Permutation_cons_append //. }
+  Qed.
+
+  #[local] Lemma pool_quicksort_main_0_spec pool ctx scope arr i i_ xs sz :
     (0 ≤ i)%Z →
     i_ = ₊i →
-    length ns = ₊sz →
+    length xs = ₊sz →
     {{{
       pool_context pool ctx scope ∗
-      array_slice arr i_ (DfracOwn 1) (#*@{Z} ns)
+      array_slice arr i_ (DfracOwn 1) (#*@{Z} xs)
     }}}
       pool_quicksort_main_0 ctx arr #i #sz
     {{{
       RET ();
       pool_context pool ctx scope ∗
       pool_consumer pool (
-        ∃ ns',
-        ⌜ns ≡ₚ ns'⌝ ∗
-        ⌜StronglySorted (≤)%Z ns'⌝ ∗
-        array_slice arr i_ (DfracOwn 1) (#*@{Z} ns')
+        ∃ xs',
+        ⌜xs ≡ₚ xs'⌝ ∗
+        ⌜StronglySorted (≤)%Z xs'⌝ ∗
+        array_slice arr i_ (DfracOwn 1) (#*@{Z} xs')
       )
     }}}.
   Proof.
     iIntros "%Hi %Hi_ %Hsz %Φ (Hctx & Harr) HΦ".
 
-    iLöb as "HLöb" forall (ctx scope i i_ ns sz Hi Hi_ Hsz Φ).
+    iLöb as "HLöb" forall (ctx scope i i_ xs sz Hi Hi_ Hsz Φ).
 
     wp_rec. wp_pures.
     case_bool_decide; wp_pures.
 
-    - wp_apply (pool_quicksort_partition_spec with "Harr") as (ns1 p pivot ns2) "(%Hp & %Hns & %Hns1 & %Hns2 & Harr)". 1-4: done.
+    - wp_apply (pool_quicksort_partition_spec with "Harr") as (xs1 p pivot xs2) "(%Hp & %Hxs & %Hxs1 & %Hxs2 & Harr)". 1-4: done.
       iDestruct (array_slice_app3 _ [_] with "Harr") as "(Harr_1 & Harr_2 & Harr_3)".
 
       wp_apply+ (pool_async_spec
         True
         ( pool_consumer pool (
-            ∃ ns1',
-            ⌜ns1 ≡ₚ ns1'⌝ ∗
-            ⌜StronglySorted (≤)%Z ns1'⌝ ∗
-            array_slice arr i_ (DfracOwn 1) (#*@{Z} ns1')
+            ∃ xs1',
+            ⌜xs1 ≡ₚ xs1'⌝ ∗
+            ⌜StronglySorted (≤)%Z xs1'⌝ ∗
+            array_slice arr i_ (DfracOwn 1) (#*@{Z} xs1')
           )
         )
       with "[$Hctx Harr_1]") as "(Hctx & _ & Hpool_consumer_1)".
@@ -87,10 +232,10 @@ Section pool_G.
       wp_apply+ (pool_async_spec
         True
         ( pool_consumer pool (
-            ∃ ns2',
-            ⌜ns2 ≡ₚ ns2'⌝ ∗
-            ⌜StronglySorted (≤)%Z ns2'⌝ ∗
-            array_slice arr (S p) (DfracOwn 1) (#*@{Z} ns2')
+            ∃ xs2',
+            ⌜xs2 ≡ₚ xs2'⌝ ∗
+            ⌜StronglySorted (≤)%Z xs2'⌝ ∗
+            array_slice arr (S p) (DfracOwn 1) (#*@{Z} xs2')
           )
         )
       with "[$Hctx Harr_3]") as "(Hctx & _ & Hpool_consumer_2)".
@@ -98,7 +243,7 @@ Section pool_G.
         wp_apply+ ("HLöb" with "[%] [%] [%] Hctx Harr_3") as "($ & Hpool_consumer)".
         { lia. }
         { simpl_length/=. lia. }
-        { apply Permutation_length in Hns. simpl_length/= in Hns. lia. }
+        { apply Permutation_length in Hxs. simpl_length/= in Hxs. lia. }
         iEval (simpl_length/=) in "Hpool_consumer".
         iEval (rewrite -Hp Nat.add_1_r) in "Hpool_consumer".
         iFrameSteps.
@@ -108,39 +253,39 @@ Section pool_G.
       iApply "HΦ".
       iFrame.
       iApply pool_consumer_intro. iIntros "#Hpool_finished".
-      iMod (pool_consumer_finished with "Hpool_consumer_1 Hpool_finished") as "(%ns1' & %Hns1'_permutation & %Hns1'_sorted & Harr_1)".
-      iMod (pool_consumer_finished with "Hpool_consumer_2 Hpool_finished") as "(%ns2' & %Hns2'_permutation & %Hns2'_sorted & Harr_3)".
+      iMod (pool_consumer_finished with "Hpool_consumer_1 Hpool_finished") as "(%xs1' & %Hxs1'_permutation & %Hxs1'_sorted & Harr_1)".
+      iMod (pool_consumer_finished with "Hpool_consumer_2 Hpool_finished") as "(%xs2' & %Hxs2'_permutation & %Hxs2'_sorted & Harr_3)".
       iDestruct (array_slice_app3_1 with "Harr_1 Harr_2 Harr_3") as "Harr".
-      { simpl_length. apply Permutation_length in Hns1'_permutation. lia. }
-      { simpl_length/=. apply Permutation_length in Hns1'_permutation. lia. }
+      { simpl_length. apply Permutation_length in Hxs1'_permutation. lia. }
+      { simpl_length/=. apply Permutation_length in Hxs1'_permutation. lia. }
       iEval (rewrite -(fmap_app _ [_]) -fmap_app) in "Harr".
       iFrame. iPureIntro. split.
-      { rewrite -Hns1'_permutation -Hns2'_permutation //. }
+      { rewrite -Hxs1'_permutation -Hxs2'_permutation //. }
       { apply: StronglySorted_app_cons. 1,4: done.
-        - rewrite -Hns1'_permutation.
+        - rewrite -Hxs1'_permutation.
           eapply Forall_impl => //=. lia.
-        - rewrite -Hns2'_permutation //.
+        - rewrite -Hxs2'_permutation //.
       }
 
     - iDestruct (pool_consumer_intro with "[Harr]") as "Hpool_consumer". 2: iSteps.
       iIntros "_ !>".
-      iExists ns. iSteps. iPureIntro.
+      iExists xs. iSteps. iPureIntro.
       apply StronglySorted_trivial. lia.
   Qed.
-  #[local] Lemma pool_quicksort_main_1_spec pool ctx scope arr ns :
+  #[local] Lemma pool_quicksort_main_1_spec pool ctx scope arr xs :
     {{{
       pool_context pool ctx scope ∗
-      array_model arr (DfracOwn 1) (#*@{Z} ns)
+      array_model arr (DfracOwn 1) (#*@{Z} xs)
     }}}
       pool_quicksort_main_1 ctx arr
     {{{
       RET ();
       pool_context pool ctx scope ∗
       pool_consumer pool (
-        ∃ ns',
-        ⌜ns ≡ₚ ns'⌝ ∗
-        ⌜StronglySorted (≤)%Z ns'⌝ ∗
-        array_model arr (DfracOwn 1) (#*@{Z} ns')
+        ∃ xs',
+        ⌜xs ≡ₚ xs'⌝ ∗
+        ⌜StronglySorted (≤)%Z xs'⌝ ∗
+        array_model arr (DfracOwn 1) (#*@{Z} xs')
       )
     }}}.
   Proof.
@@ -160,17 +305,17 @@ Section pool_G.
     simpl_length. apply Permutation_length. done.
   Qed.
 
-  Lemma pool_quicksort_main_spec (num_dom : nat) arr ns :
+  Lemma pool_quicksort_main_spec (num_dom : nat) arr xs :
     {{{
-      array_model arr (DfracOwn 1) (#*@{Z} ns)
+      array_model arr (DfracOwn 1) (#*@{Z} xs)
     }}}
       pool_quicksort_main #num_dom arr
     {{{
-      ns'
+      xs'
     , RET ();
-      ⌜ns ≡ₚ ns'⌝ ∗
-      ⌜StronglySorted (≤)%Z ns'⌝ ∗
-      array_model arr (DfracOwn 1) (#*@{Z} ns')
+      ⌜xs ≡ₚ xs'⌝ ∗
+      ⌜StronglySorted (≤)%Z xs'⌝ ∗
+      array_model arr (DfracOwn 1) (#*@{Z} xs')
     }}}.
   Proof.
     iIntros "%Φ Harr HΦ".
@@ -180,10 +325,10 @@ Section pool_G.
 
     wp_apply+ (pool_run_spec (λ _,
       pool_consumer pool (
-        ∃ ns',
-        ⌜ns ≡ₚ ns'⌝ ∗
-        ⌜StronglySorted (≤)%Z ns'⌝ ∗
-        array_model arr (DfracOwn 1) (#*@{Z} ns')
+        ∃ xs',
+        ⌜xs ≡ₚ xs'⌝ ∗
+        ⌜StronglySorted (≤)%Z xs'⌝ ∗
+        array_model arr (DfracOwn 1) (#*@{Z} xs')
       )
     )%I with "[$Hpool_model Harr]") as (?) "(Hpool_model & Hpool_consumer)".
     { iIntros "%ctx %scope Hctx".
@@ -192,7 +337,7 @@ Section pool_G.
 
     iApply wp_fupd.
     wp_apply+ (pool_kill_spec with "[$Hpool_model]") as "#Hpool_finished".
-    iMod (pool_consumer_finished with "Hpool_consumer Hpool_finished") as "(%ns' & % & % & Harr)".
+    iMod (pool_consumer_finished with "Hpool_consumer Hpool_finished") as "(%xs' & % & % & Harr)".
     iSteps.
   Qed.
 End pool_G.
